

Exercise E1.

Let  $\mathbb{X}, \mathbb{Y}$  be two real-valued stochastic variables with finite variance. Prove the following relation:

$$\text{Cor}(\mathbb{X}, \mathbb{Y}) = 1 \Leftrightarrow V(\mathbb{X}) > 0 \text{ and } \exists \text{ constants } a, b \text{ with } b \neq 0: \mathbb{X} = a + b\mathbb{Y} \text{ with probability 1.}$$

Interpretation: If two variables have correlation 1, they essentially contribute with the same information, since one can get one directly from the other.

Hint: Start by showing that a variable with variance 0 is constant with probability 1.

**Solution:**

We start by showing that a variable with variance 0 is constant with probability 1.

Assume that  $V(\mathbb{Z}) = 0$  and put  $c = E(\mathbb{Z})$ ,  $p_0 = P(|\mathbb{Z} - c| > 0)$ . Note that

$$p_0 = P\left(\bigcap_{n=1}^{\infty} |\mathbb{Z} - c| < \frac{1}{n}\right) = \lim_{n \rightarrow \infty} P\left(|\mathbb{Z} - c| < \frac{1}{n}\right)$$

WE do a counterposed proof: Suppose that  $p_0 < 1$ , and choose an  $N$  such that  $q_N = P\left(|\mathbb{Z} - c| < \frac{1}{N}\right) < 1$ . Then

$$0 = V(\mathbb{Z}) = E((\mathbb{Z} - c)^2) \geq E\left(\frac{1}{N^2} 1_{\{|\mathbb{Z} - c| \geq \frac{1}{N}\}}\right) = \frac{1}{N^2} (1 - q_N) > 0$$

Contradiction. Thus,  $P(\mathbb{Z} = c) = 1$ .  $\square$

Now the actual proof:

“ $\Leftarrow$ ”: We start by noting that

$$V(\mathbb{Y}) = V\left(\frac{1}{b}\mathbb{X} - \frac{a}{b}\right) = V\left(\frac{1}{b}\mathbb{X}\right) = b^{-2}V(\mathbb{X}) > 0.$$

Denote the variances of  $\mathbb{X}, \mathbb{Y}$  by  $\sigma_x^2, \sigma_y^2$ , respectively, so that  $\sigma_x^2 = b^2\sigma_y^2$ . Now,

$$\text{Cov}(\mathbb{X}, \mathbb{Y}) = \text{Cov}(a + b\mathbb{Y}, \mathbb{Y}) = b\text{Cov}(\mathbb{Y}, \mathbb{Y}) = b\sigma_y^2$$

Thus,

$$\text{Cor}(\mathbb{X}, \mathbb{Y}) = \frac{\text{Cov}(\mathbb{X}, \mathbb{Y})}{\sqrt{\sigma_x^2 \sigma_y^2}} = \frac{b \sigma_y^2}{\sqrt{b^2 \sigma_y^2 \sigma_y^2}} = 1.$$

“ $\Rightarrow$ ”: First observe that  $V(\mathbb{X}) > 0$  and  $V(\mathbb{Y}) > 0$  simply from the fact that  $\text{Cor}(\mathbb{X}, \mathbb{Y})$  is well defined.

Denote the covariance between  $\mathbb{X}$  and  $\mathbb{Y}$  by  $\sigma_{xy}$ . Now,

$$1 = \text{cor}(\mathbb{X}, \mathbb{Y}) = \frac{\sigma_{xy}}{\sigma_x \sigma_y},$$

So that

$$\sigma_{xy} = \sigma_x \sigma_y.$$

Now, define  $\mathbb{Z} = \mathbb{X} - \frac{\sigma_x}{\sigma_y} \mathbb{Y}$ , and note that

$$\begin{aligned} V(\mathbb{Z}) &= V\left(\mathbb{X} - \frac{\sigma_x}{\sigma_y} \mathbb{Y}\right) = \text{Cov}\left(\mathbb{X} - \frac{\sigma_x}{\sigma_y} \mathbb{Y}, \mathbb{X} - \frac{\sigma_x}{\sigma_y} \mathbb{Y}\right) \\ &= \text{Cov}(\mathbb{X}, \mathbb{X}) + \frac{\sigma_x^2}{\sigma_y^2} \text{Cov}(\mathbb{Y}, \mathbb{Y}) - 2 \frac{\sigma_x}{\sigma_y} \text{Cov}(\mathbb{X}, \mathbb{Y}) \\ &= \sigma_x^2 + \frac{\sigma_x^2}{\sigma_y^2} \sigma_y^2 - 2 \frac{\sigma_x}{\sigma_y} \sigma_{xy} \\ &= \sigma_x^2 + \sigma_x^2 - 2 \frac{\sigma_x}{\sigma_y} \sigma_x \sigma_y = 0 \end{aligned}$$

$\mathbb{Z}$  is therefore constant with probability 1. Take  $a = E(\mathbb{Z})$ ,  $b = \frac{\sigma_x}{\sigma_y} \neq 0$ . Then with probability 1,

$$\mathbb{X} = \mathbb{X} - \frac{\sigma_x}{\sigma_y} \mathbb{Y} + \frac{\sigma_x}{\sigma_y} \mathbb{Y} = \mathbb{Z} + \frac{\sigma_x}{\sigma_y} \mathbb{Y} = a + b \mathbb{Y}. \square$$